clightplus_examples/xorlist/xorlistall01proof.v
@@ -1,36 +1,82 @@
+Require Import CoqlibCCR.
+Require Import Any.
+Require Import STS.
+Require Import Behavior.
+Require Import ModSem.
+Require Import SimModSem.
+Require Import PCM.
+Require Import HoareDef.
+Require Import STB.
+Require Import ClightPlusSkel ClightPlusExprgen ClightPlusgen.
+Require Import ClightPlusMem0 ClightPlusMem1 ClightPlusMemAux.
+Require Import CProofMode CIProofMode.
+Require Import xorlist.
+Require Import xorlistall0.
+Require Import xorlistall1.
+Require Import xorlist1.
+Require Import PtrofsArith.
+From Coq Require Import Program.
+From compcert Require Import Clightdefs.
 
-  Section SIMFUNS.
+Require Import ClightPlusMem01Proof.
+Require Import xorlist01proof.
+Require Import main01proof.
+
+Section PROOF.
+
+  Import ClightPlusMem1.
+
+  Context `{@GRA.inG pointstoRA Σ}.
+  Context `{@GRA.inG allocatedRA Σ}.
+  Context `{@GRA.inG blocksizeRA Σ}.
+  Context `{@GRA.inG blockaddressRA Σ}.
+  
+  Variable GlobalStb : Sk.t -> gname -> option fspec.
+  Hypothesis MEMINCL : forall sk, stb_incl (to_stb MemStb) (GlobalStb sk).
+  Hypothesis STBINCL : forall sk, stb_incl (to_stb xorStb) (GlobalStb sk).
+
   Variable xorlink : Clight.program.
   Variable xormod : Mod.t.
-  Hypothesis VALID_link : xorlist0._xor = Some xorlink.
+  Hypothesis VALID_link : xorlistall0._xor = Some xorlink.
   Hypothesis VALID_comp : compile xorlink "xorlist" = Errors.OK xormod.
   Let mfsk : Sk.t := [("malloc", Gfun (F:=Clight.fundef) (V:=type) (Ctypes.External EF_malloc (Tcons tulong Tnil) (tptr tvoid) cc_default)); ("free", Gfun (Ctypes.External EF_free (Tcons (tptr tvoid) Tnil) tvoid cc_default))].
-  (* Require Import ClightPlusMem01Proof. *)
 
-  Variable xor0 : Mod.t.
-  Hypothesis VALID : xorlist0._xor = Errors.OK xor0.
+  (* Variable xor0 : Mod.t.
+  Hypothesis VALID : xorlist0._xor = Errors.OK xor0. *)
 
-  Theorem correct : refines2 [xormod; ClightPlusMem0.Mem mfsk] [xorlistall1.xor xormod GlobalStb; ClightPlusMem1.Mem mfsk].
+  Theorem correct : refines2 [xormod; ClightPlusMem0.Mem mfsk] [xorlistall1.xorAllWrapped GlobalStb; ClightPlusMem1.Mem mfsk].
   Proof.
     eapply adequacy_local_strong_l. econs; cycle 1.
-    { econs; [ss|]. econs; ss. }
+    { simpl map. econs; [|econs; refl].
+      unfold xor_sk, xor. rewrite VALID_link. rewrite VALID_comp. et. }
     i. econs; cycle 1.
     { econs; [|ss]. apply correct_mod; et. inv SKINCL. inv H6. ss. }
-    unfold _xor, compile, get_sk in VALID.
-    destruct Pos.eq_dec; [|clarify].
-    destruct Coqlib.list_norepet_dec; ss. des_ifs_safe.
-    econstructor 1 with (wf := wf) (le := top2); et; ss; cycle 1.
+    hexploit sim_delete_tl; et. { inv SKINCL. inv H6. et. } i. rename H3 into sim_delete_tl.
+    hexploit sim_delete_hd; et. { inv SKINCL. inv H6. et. } i. rename H3 into sim_delete_hd.
+    hexploit sim_add_hd; et. { inv SKINCL. inv H6. et. } i. rename H3 into sim_add_hd.
+    hexploit sim_add_tl; et. { inv SKINCL. inv H6. et. } i. rename H3 into sim_add_tl.
+    hexploit sim_main; et. { inv SKINCL. et. } { inv SKINCL. inv H6. et. } i. rename H3 into sim_main.
+    eassert (_xor = _).
+    { unfold _xor. vm_compute (Linking.link _ _). reflexivity. }
+    rewrite H3 in *. clear H3. destruct Ctypes.link_build_composite_env. destruct a.
+    inversion VALID_link. clear VALID_link. subst.
+    clear a.
+    set (compile _ _) in VALID_comp.
+    eassert (r = Errors.OK _).
+    { reflexivity. }
+    rewrite H3 in *. clear r H3.
+    inversion VALID_comp. clear VALID_comp. subst. ss.
+    econstructor 1 with (wf := xorlist01proof.wf) (le := top2); et; ss; cycle 1.
     { eexists. econs. apply to_semantic. iIntros. et. }
     (* each functions has simulation relation *)
-    econs; cycle 1.
-    econs; cycle 1.
-    econs; cycle 1.
-    econs; cycle 1.
-    econs; et.
-    all: des_ifs; inv SKINCL; inv H6; ss.
-    - eapply sim_delete_tl; et.
-    - eapply sim_delete_hd; et.
-    - eapply sim_add_tl; et.
-    - eapply sim_add_hd; et.
+    unfold get_ce. simpl prog_comp_env.
+    econs. { apply sim_add_hd. }
+    econs. { apply sim_add_tl. }
+    econs. { apply sim_main. }
+    econs. { apply sim_delete_hd. }
+    econs. { apply sim_delete_tl. }
+    econs.
     Unshelve. exact tt.
   Qed.
+
+End PROOF.
